Concrete_Semantics_7.thy
@@ -1,0 +1,199 @@
+theory Concrete_Semantics_7
+  imports Main "~~/src/HOL/IMP/Com" "HOL-IMP.Star"
+begin
+
+(* "~~/src/HOL/IMP/Com" *)
+inductive
+  big_step :: "com \<times> state \<Rightarrow> state \<Rightarrow> bool" (infix "\<Rightarrow>" 55)
+where
+Skip: "(SKIP,s) \<Rightarrow> s" |
+Assign: "(x ::= a,s) \<Rightarrow> s(x := aval a s)" |
+Seq: "\<lbrakk> (c\<^sub>1,s\<^sub>1) \<Rightarrow> s\<^sub>2;  (c\<^sub>2,s\<^sub>2) \<Rightarrow> s\<^sub>3 \<rbrakk> \<Longrightarrow> (c\<^sub>1;;c\<^sub>2, s\<^sub>1) \<Rightarrow> s\<^sub>3" |
+IfTrue: "\<lbrakk> bval b s;  (c\<^sub>1,s) \<Rightarrow> t \<rbrakk> \<Longrightarrow> (IF b THEN c\<^sub>1 ELSE c\<^sub>2, s) \<Rightarrow> t" |
+IfFalse: "\<lbrakk> \<not>bval b s;  (c\<^sub>2,s) \<Rightarrow> t \<rbrakk> \<Longrightarrow> (IF b THEN c\<^sub>1 ELSE c\<^sub>2, s) \<Rightarrow> t" |
+WhileFalse: "\<not>bval b s \<Longrightarrow> (WHILE b DO c,s) \<Rightarrow> s" |
+WhileTrue:
+"\<lbrakk> bval b s\<^sub>1;  (c,s\<^sub>1) \<Rightarrow> s\<^sub>2;  (WHILE b DO c, s\<^sub>2) \<Rightarrow> s\<^sub>3 \<rbrakk> 
+\<Longrightarrow> (WHILE b DO c, s\<^sub>1) \<Rightarrow> s\<^sub>3"
+
+schematic_goal ex : "(''x'' ::= N 5;; ''y'' ::= V ''x'', s) \<Rightarrow> ?t"
+  apply(rule Seq)
+   apply(rule Assign)
+  apply simp
+  apply(rule Assign)
+  done
+thm ex[simplified]
+
+code_pred big_step .
+
+values "{t. (SKIP, \<lambda>_. 0) \<Rightarrow> t}"
+values "{map t [''x''] |t. (SKIP, <''x'' := 42>) \<Rightarrow> t}"
+
+values "{map t [''x''] |t. (''x'' ::= N 2, <''x'' := 42>) \<Rightarrow> t}"
+values "{map t [''x'', ''y''] |t. (''x'' ::= N 2, \<lambda>_.0) \<Rightarrow> t}"
+
+(* the following inverted rules(inductive cases) are needed to prove. *)
+inductive_cases SkipE[elim!]: "(SKIP,s) \<Rightarrow> t"
+thm SkipE
+inductive_cases AssignE[elim!]: "(x ::= a,s) \<Rightarrow> t"
+thm AssignE
+inductive_cases SeqE[elim!]: "(c1;;c2,s1) \<Rightarrow> s3"
+thm SeqE
+inductive_cases IfE[elim!]: "(IF b THEN c1 ELSE c2,s) \<Rightarrow> t"
+thm IfE
+inductive_cases WhileE[elim]: "(WHILE b DO c,s) \<Rightarrow> t"
+thm WhileE
+
+declare big_step.intros [intro]
+thm big_step.induct
+
+lemma "(IF b THEN SKIP ELSE SKIP, s) \<Rightarrow> t \<Longrightarrow> t = s"
+  by blast
+
+lemma assumes "(IF b THEN SKIP ELSE SKIP, s) \<Rightarrow> t"
+  shows "t = s"
+proof-
+  from assms show ?thesis
+  proof cases
+  case IfTrue
+  then show ?thesis 
+    by auto
+next
+  case IfFalse
+  then show ?thesis  by blast
+qed
+qed
+
+lemma Seq_assoc:
+  "(c1;; c2;; c3, s) \<Rightarrow> s' \<longleftrightarrow> (c1;; (c2;; c3), s) \<Rightarrow> s'"
+proof
+  assume "(c1;; c2;; c3, s) \<Rightarrow> s'"
+  then obtain s1 s2 where
+c1: "(c1, s) \<Rightarrow> s1" and
+c2: "(c2, s1) \<Rightarrow> s2" and
+c3: "(c3, s2) \<Rightarrow> s'" 
+    by blast
+    from c2 c3 have "(c2;; c3, s1) \<Rightarrow> s'" 
+      using Seq by auto
+  show "(c1;; (c2;; c3), s) \<Rightarrow> s'" 
+    using Seq \<open>(c2;; c3, s1) \<Rightarrow> s'\<close> c1 by blast
+next
+  assume "(c1;; (c2;; c3), s) \<Rightarrow> s'"
+
+  then show  "(c1;; c2;; c3, s) \<Rightarrow> s'" 
+    by (meson Seq SeqE)
+qed
+
+abbreviation
+  equiv_c :: "com \<Rightarrow> com \<Rightarrow> bool" (infix "\<sim>" 50) where
+  "c \<sim> c' \<equiv> (\<forall>s t. (c,s) \<Rightarrow> t  =  (c',s) \<Rightarrow> t)"
+
+lemma while_unfold:
+  "(WHILE b DO c) \<sim> (IF b THEN c;; WHILE b DO c ELSE SKIP)"
+  by blast
+
+lemma unfold_while:
+  "(WHILE b DO c)\<sim>(IF b THEN c;; WHILE b DO c ELSE SKIP)" (is "?w \<sim> ?iw")
+proof -
+  have "(?iw, s) \<Rightarrow> t" if assm: "(?w, s) \<Rightarrow> t" for s t
+  proof -
+    from assm show ?thesis
+    proof cases
+      case WhileFalse
+      then show ?thesis 
+        by (simp add: IfFalse Skip)
+    next
+      case (WhileTrue s\<^sub>2)
+      then show ?thesis 
+        using IfTrue Seq by auto
+    qed
+  qed
+  moreover 
+  have  "(?w, s) \<Rightarrow> t" if assm: "(?iw, s) \<Rightarrow> t" for s t
+  proof -
+    from assm show ?thesis
+    proof cases
+      case IfTrue
+      then show ?thesis 
+        using WhileTrue by auto
+    next
+      case IfFalse
+      then show ?thesis 
+        using WhileFalse by blast
+    qed
+  qed
+  ultimately
+  show ?thesis 
+    by blast
+qed
+
+lemma triv_if:
+  "(IF b THEN c ELSE c) \<sim> c"
+  by blast
+
+lemma commute_if:
+  "(IF b1 THEN (IF b2 THEN c11 ELSE c12) ELSE c2) 
+   \<sim> 
+   (IF b2 THEN (IF b1 THEN c11 ELSE c2) ELSE (IF b1 THEN c12 ELSE c2))"
+  by blast
+
+
+(* Q. What is big_step.induct[split_format(complete)]?
+A. The proof of Lemma 7.6
+requires the advanced form of rule induction described in Section 5.4.6 because
+the big-step premise in the lemma involves not just variables but the
+proper term WHILE b DO c.
+ *)
+lemma sim_while_cong_aux:
+  "\<lbrakk>(WHILE b DO c,s) \<Rightarrow> t ; c \<sim> c'\<rbrakk> \<Longrightarrow>  (WHILE b DO c',s) \<Rightarrow> t"
+  apply(induction "WHILE b DO c" s t arbitrary: b c rule:  big_step.induct[split_format(complete)])
+   apply (simp add: WhileFalse)
+  by blast
+
+
+lemma sim_while_cong: "c \<sim> c' \<Longrightarrow> WHILE b DO c \<sim> WHILE b DO c'"
+  using sim_while_cong_aux by auto
+
+lemma sim_refl:  "c \<sim> c" 
+  by simp
+lemma sim_sym:   "(c \<sim> c') = (c' \<sim> c)" 
+  by auto
+lemma sim_trans: "c \<sim> c' \<Longrightarrow> c' \<sim> c'' \<Longrightarrow> c \<sim> c''" 
+  by simp
+
+theorem big_step_determ: "\<lbrakk> (c,s) \<Rightarrow> t; (c,s) \<Rightarrow> u \<rbrakk> \<Longrightarrow> u = t"
+  apply(induction arbitrary:u rule: big_step.induct)
+  apply (blast+)
+  done
+
+theorem "(c, s) \<Rightarrow> t \<Longrightarrow> (c, s) \<Rightarrow> t' \<Longrightarrow> t' = t"
+proof (induction arbitrary: t' rule: big_step.induct)
+  case (Skip s)
+  then show ?case 
+    by auto
+next
+  case (Assign x a s)
+  then show ?case 
+    by auto
+next
+  case (Seq c\<^sub>1 s\<^sub>1 s\<^sub>2 c\<^sub>2 s\<^sub>3)
+  then show ?case 
+    by blast
+next
+  case (IfTrue b s c\<^sub>1 t c\<^sub>2)
+  then show ?case 
+    by blast
+next
+  case (IfFalse b s c\<^sub>2 t c\<^sub>1)
+  then show ?case 
+    by blast
+next
+  case (WhileFalse b s c)
+  then show ?case 
+    by auto
+next
+  case (WhileTrue b s\<^sub>1 c s\<^sub>2 s\<^sub>3)
+  then show ?case 
+    by blast
+qed
+
