Concrete_Semantics_7_Ex.thy
@@ -1,0 +1,307 @@
+theory Concrete_Semantics_7_Ex
+  imports Main "~~/src/HOL/IMP/Com" "HOL-IMP.Big_Step" "HOL-IMP.Small_Step"
+begin
+
+(* Exercise 7.1. *)
+
+fun assigned :: "com \<Rightarrow> vname set" where
+"assigned SKIP = {}" |
+"assigned (v ::= va) = {v}"| 
+"assigned (v;; va) = assigned v \<union> assigned va " |
+"assigned (IF v THEN va ELSE vb) = assigned va \<union> assigned vb" | 
+"assigned (WHILE v DO va) = assigned va"
+
+lemma "\<lbrakk>(c, s) \<Rightarrow> t; x \<notin> assigned c\<rbrakk> \<Longrightarrow> s x = t x"
+proof(induction rule:big_step_induct)
+  case (Skip s)
+  then show ?case 
+    by simp
+next
+  case (Assign x a s)
+  then show ?case 
+    by simp
+next
+  case (Seq c\<^sub>1 s\<^sub>1 s\<^sub>2 c\<^sub>2 s\<^sub>3)
+  then show ?case 
+    by simp
+next
+  case (IfTrue b s c\<^sub>1 t c\<^sub>2)
+  then show ?case by simp
+next
+  case (IfFalse b s c\<^sub>2 t c\<^sub>1)
+  then show ?case by simp
+next
+  case (WhileFalse b s c)
+  then show ?case by simp
+next
+  case (WhileTrue b s\<^sub>1 c s\<^sub>2 s\<^sub>3)
+  then show ?case by simp
+qed
+
+(* Exercise 7.2. *)
+fun skip :: "com \<Rightarrow> bool" where
+"skip SKIP = True" |
+"skip (v ::= va) = False" |
+"skip (v;; va) = (skip v \<and> skip va)" |
+"skip (IF v THEN va ELSE vb) = (skip va \<and> skip vb)" |
+"skip (WHILE v DO va) = False"
+
+lemma "skip c \<Longrightarrow> c \<sim> SKIP"
+proof(induction c)
+case SKIP
+  then show ?case 
+    by simp
+next
+  case (Assign x1 x2)
+  then show ?case by simp
+next
+  case (Seq c1 c2)
+  then show ?case 
+    by fastforce
+next
+  case (If x1 c1 c2)
+  then show ?case 
+    by (meson Big_Step.IfE big_step.IfFalse big_step.IfTrue skip.simps(4))
+next
+  case (While x1 c)
+  then show ?case 
+    by simp
+qed
+
+(* Exercise 7.3. *)
+fun deskip :: "com \<Rightarrow> com" where
+"deskip SKIP = SKIP" |
+(* b is aexp so not to do deskip*)
+"deskip (a ::= b) = a ::= b" |
+"deskip (a;; b) = (if deskip a = SKIP then deskip b else 
+  (if deskip b = SKIP then deskip a 
+    else deskip a;; deskip b))" |
+"deskip (IF a THEN b ELSE c) = IF a THEN deskip b ELSE deskip c" |
+"deskip (WHILE a DO b) = WHILE a DO deskip b"
+
+value "deskip (SKIP;; WHILE b DO (x ::= a;; SKIP))"
+
+lemma "deskip c \<sim> c"
+proof(induction c)
+case SKIP
+  then show ?case by simp
+next
+  case (Assign x1 x2)
+  then show ?case by simp
+next
+  case (Seq c1 c2)
+  then have "(c1 ;; c2) \<sim> (deskip c1;; deskip c2)" 
+    by blast
+  moreover have " deskip (c1;; c2) \<sim> (deskip c1;; deskip c2)" 
+    by auto
+(* deskip (c1;; c2) \sim (deskip c1;; deskip c2) \sim (c1;; c2) *)
+  ultimately show ?case by auto
+next
+  case (If x1 c1 c2)
+  then show ?case 
+    by auto
+next
+  case (While x1 c)
+
+  then show ?case 
+    using sim_while_cong by auto
+qed
+
+inductive astep :: "aexp * state \<Rightarrow> aexp \<Rightarrow> bool" (infix "\<leadsto>" 50) where
+"(V x , s) \<leadsto>  N (s x )" |
+"(Plus (N i) (N j ), s) \<leadsto> N (i + j )" |
+"(x2, s) \<leadsto> a2 \<Longrightarrow> (Plus x1 x2, s) \<leadsto> Plus x1 a2" |
+"(x1, s) \<leadsto> a1 \<Longrightarrow> (Plus x1 (N j), s) \<leadsto> Plus a1 (N j)"
+
+
+lemma "(a, s) \<leadsto> a' \<Longrightarrow> aval a s = aval a' s"
+proof (induction rule: astep.induct[split_format(complete)])
+  fix x s 
+  show "aval (V x) s = aval (N (s x)) s" 
+    by simp
+
+  fix i j s
+  show "aval (Plus (N i) (N j)) s = aval (N (i + j)) s" 
+    by simp
+
+  fix x2 s a2 x1
+  assume "aval x2 s = aval a2 s"
+  then show "aval (Plus x1 x2) s = aval (Plus x1 a2) s" 
+    by simp
+
+  fix x1 s a1 j
+  assume "aval x1 s = aval a1 s"
+  then show "aval (Plus x1 (N j)) s = aval (Plus a1 (N j)) s" 
+    by simp 
+qed
+
+lemma "IF And b1 b2 THEN c1 ELSE c2 \<sim>
+IF b1 THEN IF b2 THEN c1 ELSE c2 ELSE c2"(is "?left \<sim> ?right")
+proof -
+  have "(?left,s) \<Rightarrow> t \<Longrightarrow> (?right, s) \<Rightarrow> t"  for s t
+  proof -
+    assume "(?left, s) \<Rightarrow> t"
+    show "(?right, s) \<Rightarrow> t" 
+      using IfTrue \<open>(IF And b1 b2 THEN c1 ELSE c2, s) \<Rightarrow> t\<close> by fastforce
+  qed
+  moreover have "(?right, s) \<Rightarrow> t \<Longrightarrow> (?left,s) \<Rightarrow> t"  for s t
+  proof -
+    assume "(?right, s) \<Rightarrow> t" 
+    show "(?left, s) \<Rightarrow> t" 
+      using \<open>(IF b1 THEN IF b2 THEN c1 ELSE c2 ELSE c2, s) \<Rightarrow> t\<close> by auto
+  qed
+  ultimately show ?thesis 
+    by blast 
+qed
+  
+(* obviously false*)
+
+(* 
+  then show False by (induction rule: big_step_induct)
+Failed to finish proof\<^here>:
+goal (3 subgoals):
+ 1. \<And>s. False
+ 2. \<And>x a s. False
+ 3. \<And>b s c. \<not> bval b s \<Longrightarrow> False
+
+  then show False by (induction "WHILE (Bc True) DO WHILE (Bc False) DO SKIP" s s rule: big_step_induct)
+Failed to finish proof\<^here>:
+goal (1 subgoal):
+ 1. \<And>s. \<not> bval (Bc True) s \<Longrightarrow> False
+ *)
+lemma "\<not> (\<forall> b1 b2 c. WHILE And b1 b2 DO c \<sim> WHILE b1 DO WHILE b2 DO c)"(is "\<not> ?p")
+proof 
+  assume assm: ?p
+  have 1: "WHILE And (Bc True) (Bc False) DO SKIP \<sim> WHILE (Bc True) DO WHILE (Bc False) DO SKIP"
+    using assm by simp
+  have 2: "(WHILE And (Bc True) (Bc False) DO SKIP, s) \<Rightarrow> s" by auto
+  have 3: "(WHILE (Bc True) DO WHILE (Bc False) DO SKIP, s) \<Rightarrow> s" 
+    using "2" assm by auto
+  then show False 
+    by (induction "WHILE (Bc True) DO WHILE (Bc False) DO SKIP" s s rule: big_step_induct, simp)
+qed
+
+lemma temination_of_while: "(WHILE b DO c, s) \<Rightarrow> t \<Longrightarrow> \<not> bval b t"
+  apply(induction "WHILE b DO c" s t rule: big_step_induct )
+   apply simp
+  by simp
+
+
+  
+(*
+It is easy to show there is a proof of left to right.
+However, it is difficult to construct proof.
+The following method is failed to calculate:
+    assume assm: "(?left, s) \<Rightarrow> t"
+    then show "(?left;;?q, s) \<Rightarrow> t"
+      by (induction "WHILE Or b1 b2 DO c" s t rule: big_step_induct)
+.
+*)
+lemma "WHILE Not (And (Not b1) (Not b2)) DO c \<sim> WHILE Not (And (Not b1) (Not b2)) DO c;; WHILE b1 DO c"(is "?left \<sim> ?left;;?q")
+proof -
+  have "(?left,s) \<Rightarrow> t \<Longrightarrow> (?left;;?q, s) \<Rightarrow> t"  for s t
+  proof -
+    assume assm: "(?left, s) \<Rightarrow> t"
+    show "(?left;;?q, s) \<Rightarrow> t"
+      using Seq WhileFalse assm temination_of_while by fastforce
+  qed
+  moreover have "(?left;;?q, s) \<Rightarrow> t \<Longrightarrow> (?left,s) \<Rightarrow> t"  for s t
+  proof -
+    assume "(?left;;?q, s) \<Rightarrow> t" 
+    show "(?left, s) \<Rightarrow> t"
+      by (metis SeqE \<open>(WHILE bexp.Not (And (bexp.Not b1) (bexp.Not b2)) DO c;; WHILE b1 DO c, s) \<Rightarrow> t\<close> big_step_determ calculation)
+  qed
+  ultimately show ?thesis 
+    by blast 
+qed
+
+(* Exercise 7.6. *)
+definition Do :: "com \<Rightarrow> bexp \<Rightarrow> com" ("DO _ WHILE _"  [0, 61] 61) where
+"DO c WHILE b = c ;; WHILE b DO c" 
+
+fun dewhile :: "com \<Rightarrow> com" where
+"dewhile SKIP = SKIP" |
+(* b is aexp so not to do deskip*)
+"dewhile (a ::= b) = a ::= b" |
+"dewhile (a;; b) = (dewhile a;; dewhile b)" |
+"dewhile (IF a THEN b ELSE c) = IF a THEN dewhile b ELSE dewhile c" |
+"dewhile (WHILE a DO b) = IF a THEN (DO dewhile b WHILE a) ELSE SKIP "
+
+lemma "dewhile c \<sim> c"(is "?left \<sim> ?right")
+proof (induction c)
+  case SKIP
+then show ?case 
+  by simp
+next
+  case (Assign x1 x2)
+  then show ?case 
+    by simp
+next
+  case (Seq c1 c2)
+  then show ?case 
+    by auto
+next
+  case (If x1 c1 c2)
+  then show ?case 
+    by auto
+next
+  case (While x1 c)
+  then show ?case 
+    using Do_def sim_while_cong while_unfold by auto
+qed
+
+(* Exercise 7.7. *)
+
+lemma assumes "C 0 = c;; d" 
+  and "\<forall>n. (C n, S n) \<rightarrow> (C (Suc n), S (Suc n))"
+  shows "(\<forall> n.  \<exists>c1 c2.
+      C n = c1;; d \<and>
+      C (Suc n) = c2;; d \<and> (c1, S n) \<rightarrow> (c2, S (Suc n))) \<or>
+      (\<exists> k. C k = SKIP;; d)"(is "(?P) \<or> ?Q")
+proof cases
+  assume "?Q"
+  then show ?thesis 
+    by simp
+next
+  assume "\<not> ?Q"
+  {fix i
+    have "\<exists>c1 c2.
+        C i = c1;; d \<and>
+        C (Suc i) = c2;; d \<and> 
+        (c1, S i) \<rightarrow> (c2, S (Suc i))" 
+    proof (induction i)
+      case 0
+      then show ?case 
+        by (metis Pair_inject Small_Step.SeqE \<open>\<nexists>k. C k = SKIP;; d\<close> assms(1) assms(2))
+    next
+      case (Suc i)
+      then show ?case 
+        by (metis Pair_inject Small_Step.SeqE \<open>\<nexists>k. C k = SKIP;; d\<close> assms(2))
+    qed}
+    then have ?P 
+      by auto
+  then show ?thesis by simp
+qed
+
+(*
+
+  assume "\<not> ?P"
+  then obtain n where
+    "\<forall> c1 c2. C n \<noteq> c1;; d \<or> 
+    C (Suc n) \<noteq> c2;; d \<or>
+    \<not> ((c1, S n) \<rightarrow> (c2, S (Suc n)))" 
+    by auto
+
+To show ?thesis, I want the case 
+- "c2 = SKIP" and 
+- "C (Suc n) = c2;; d"
+, so, it is needed to show that 
+- "C n \<noteq> c1;; d"
+? ? ? ?
+CRAZY.
+REMIND.
+*)
+
+
+
+end
